[WFU] Some reorganization

WFU.v
@@ -1,44 +1,54 @@
 Import EqNotations.
+
 Unset Universe Checking.
+Inductive U : Prop := u (X : Prop) (f : X -> U) : U.
+Set Universe Checking.
 
-Inductive U : Prop := u { X : Prop ; f : X -> U }.
-
-Inductive WF : U -> Prop :=
-| wf : forall X f, (forall x, WF (f x)) -> WF (u X f).
+Definition injU [u1 u2 : U] (p : u1 = u2) :
+  match u1, u2 with
+  | u X1 f1, u X2 f2 =>
+    exists (q : X1 = X2),
+      rew [fun Z => Z -> U] q in f1 = f2
+  end :=
+  rew dependent p in
+  match u1 with
+  | u _ _ => ex_intro _ eq_refl eq_refl
+  end.
 
 Definition loop : U :=
   u U (fun x => x).
 
-Definition invU [u1 u2 : U] (p : u1 = u2) :
-  exists (q : u1.(X) = u2.(X)),
-    rew [fun Z => Z -> U] q in u1.(f) = u2.(f) :=
-  rew dependent p in ex_intro _ eq_refl eq_refl.
-
-Fixpoint nwf' (wfl : WF loop) : False :=
-  match wfl in WF u' return loop = u' -> False with
-  | wf _ f h => fun p => let (q , r) := invU p in
-    (rew dependent [fun _ q => forall f,
-      rew [fun Z => Z -> U] q in (fun x => x) = f
-      -> (forall x, WF (f x))
-      -> False] q
-    in fun _ r =>
-      rew [fun f => (forall x, WF (f x)) -> False] r
-      in fun h => nwf' (h loop)) f r h
-  end eq_refl.
-
-Require Import Coq.Program.Equality.
-Lemma nwf (u : U) (p : u = loop) (wfl : WF u) : False.
-Proof.
-  dependent induction wfl.
-  apply invU in p as [q r].
-  simpl in q. subst.
-  simpl in r. subst.
-  eapply H0. reflexivity.
-Qed.
+Inductive WF : U -> Prop :=
+| wf : forall X f, (forall x, WF (f x)) -> WF (u X f).
 
 Fixpoint wfU (u : U) : WF u :=
   match u with
   | u X f => wf X f (fun x => wfU (f x))
   end.
 
-Definition false : False := nwf loop eq_refl (wfU loop).
+Require Import Coq.Program.Equality.
+
+Lemma nwf' (u : U) (p : u = loop) (wfl : WF u) : False.
+Proof.
+  dependent induction wfl.
+  apply injU in p as [q r].
+  simpl in q. subst.
+  simpl in r. subst.
+  eapply H0. reflexivity.
+Qed.
+
+Definition nwf (wfl : WF loop) : False := nwf' loop eq_refl wfl.
+
+Fixpoint nwf'' (wfl : WF loop) : False :=
+  match wfl in WF u' return loop = u' -> False with
+  | wf _ f h => fun p => let (q , r) := injU p in
+    (rew dependent [fun _ q => forall f,
+      rew [fun Z => Z -> U] q in (fun x => x) = f
+      -> (forall x, WF (f x))
+      -> False] q
+    in fun _ r =>
+      rew [fun f => (forall x, WF (f x)) -> False] r
+      in fun h => nwf'' (h loop)) f r h
+  end eq_refl.
+
+Definition false : False := nwf (wfU loop).
